Update linking Pis and example files

dimsum/iris/combinators.v
@@ -675,45 +675,47 @@ Section link.
 
   Definition tgt_link_left_constP R {m1 m2 : mod_trans (io_event EV)}
     (Π : option (io_event EV) → link_case EV * S * m_state m1 * m_state m2 → iProp Σ)
-    (γ_s γ_σ2 γ_oe : gname) : option (io_event EV) → m_state m1 → iProp Σ :=
+    (γ_s γ_σ1 γ_σ2 γ_oe : gname) : option (io_event EV) → m_state m1 → iProp Σ :=
     λ κ σ1',
       (∀ s σ2 oe,
-         γ_s ⤳ s -∗ γ_σ2 ⤳ σ2 -∗ γ_oe ⤳ oe -∗
+         γ_s ⤳ s -∗ γ_σ1 ⤳@{m_state m1} - -∗ γ_σ2 ⤳ σ2 -∗ γ_oe ⤳ oe -∗
          match oe with
          | Some e => tgt_link_recv_leftP R Π s σ2 e κ σ1'
          | None => tgt_link_run_leftP R Π s σ2 κ σ1'
          end)%I.
 
-  Lemma sim_tgt_link_left_const_recv γ_s γ_σ2 γ_oe R m1 m2 s σ1 σ2 e Π :
+  Lemma sim_tgt_link_left_const_recv γ_s γ_σ1 γ_σ2 γ_oe R m1 m2 s σ1 σ2 e Π :
     γ_s ⤳@{S} - -∗
+    γ_σ1 ⤳@{m_state m1} - -∗
     γ_σ2 ⤳@{m_state m2} - -∗
     γ_oe ⤳@{option EV}- -∗
-    (γ_s ⤳ s -∗ γ_σ2 ⤳ σ2 -∗ γ_oe ⤳ Some e -∗ σ1 ≈{m1}≈>ₜ tgt_link_left_constP R Π γ_s γ_σ2 γ_oe) -∗
+    (γ_s ⤳ s -∗ γ_σ2 ⤳ σ2 -∗ γ_oe ⤳ Some e -∗ σ1 ≈{m1}≈>ₜ tgt_link_left_constP R Π γ_s γ_σ1 γ_σ2 γ_oe) -∗
     (MLFRecv SPLeft e, s, σ1, σ2) ≈{link_trans R m1 m2}≈>ₜ Π.
   Proof.
-    iIntros "Hγ_s Hγ_σ2 Hγ_oe Hsim".
+    iIntros "Hγ_s Hγ_σ1 Hγ_σ2 Hγ_oe Hsim".
     iMod (mstate_var_split γ_s with "Hγ_s") as "[??]".
     iMod (mstate_var_split γ_σ2 with "Hγ_σ2") as "[??]".
     iMod (mstate_var_split γ_oe with "Hγ_oe") as "[??]".
     iApply sim_tgt_link_recv_left. iSpecialize ("Hsim" with "[$] [$] [$]").
     iApply (sim_gen_wand with "Hsim"). iIntros (??) "Hsim".
-    iApply ("Hsim" with "[$] [$] [$]").
+    iApply ("Hsim" with "[$] [$] [$] [$]").
   Qed.
 
-  Lemma sim_tgt_link_left_const_run γ_s γ_σ2 γ_oe R m1 m2 s σ1 σ2 Π :
+  Lemma sim_tgt_link_left_const_run γ_s γ_σ1 γ_σ2 γ_oe R m1 m2 s σ1 σ2 Π :
     γ_s ⤳@{S} - -∗
+    γ_σ1 ⤳@{m_state m1} - -∗
     γ_σ2 ⤳@{m_state m2} - -∗
     γ_oe ⤳@{option EV}- -∗
-    (γ_s ⤳ s -∗ γ_σ2 ⤳ σ2 -∗ γ_oe ⤳ (@None EV) -∗ σ1 ≈{m1}≈>ₜ tgt_link_left_constP R Π γ_s γ_σ2 γ_oe) -∗
+    (γ_s ⤳ s -∗ γ_σ2 ⤳ σ2 -∗ γ_oe ⤳ (@None EV) -∗ σ1 ≈{m1}≈>ₜ tgt_link_left_constP R Π γ_s γ_σ1 γ_σ2 γ_oe) -∗
     (MLFRun (Some SPLeft), s, σ1, σ2) ≈{link_trans R m1 m2}≈>ₜ Π.
   Proof.
-    iIntros "Hγ_s Hγ_σ2 Hγ_oe Hsim".
+    iIntros "Hγ_s Hγ_σ1 Hγ_σ2 Hγ_oe Hsim".
     iMod (mstate_var_split γ_s with "Hγ_s") as "[??]".
     iMod (mstate_var_split γ_σ2 with "Hγ_σ2") as "[??]".
     iMod (mstate_var_split γ_oe with "Hγ_oe") as "[??]".
     iApply sim_tgt_link_run_left. iSpecialize ("Hsim" with "[$] [$] [$]").
     iApply (sim_gen_wand with "Hsim"). iIntros (??) "Hsim".
-    iApply ("Hsim" with "[$] [$] [$]").
+    iApply ("Hsim" with "[$] [$] [$] [$]").
   Qed.
 
   Definition tgt_link_run_rightP R {m1 m2 : mod_trans (io_event EV)}
@@ -820,45 +822,47 @@ Section link.
 
   Definition tgt_link_right_constP R {m1 m2 : mod_trans (io_event EV)}
     (Π : option (io_event EV) → link_case EV * S * m_state m1 * m_state m2 → iProp Σ)
-    (γ_s γ_σ1 γ_oe : gname) : option (io_event EV) → m_state m2 → iProp Σ :=
+    (γ_s γ_σ1 γ_σ2 γ_oe : gname) : option (io_event EV) → m_state m2 → iProp Σ :=
     λ κ σ2',
       (∀ s σ1 oe,
-         γ_s ⤳ s -∗ γ_σ1 ⤳ σ1 -∗ γ_oe ⤳ oe -∗
+         γ_s ⤳ s -∗ γ_σ1 ⤳ σ1 -∗ γ_σ2 ⤳@{m_state m2} - -∗ γ_oe ⤳ oe -∗
          match oe with
          | Some e => tgt_link_recv_rightP R Π s σ1 e κ σ2'
          | None => tgt_link_run_rightP R Π s σ1 κ σ2'
          end)%I.
 
-  Lemma sim_tgt_link_right_const_recv γ_s γ_σ1 γ_oe R m1 m2 s σ1 σ2 e Π :
+  Lemma sim_tgt_link_right_const_recv γ_s γ_σ1 γ_σ2 γ_oe R m1 m2 s σ1 σ2 e Π :
     γ_s ⤳@{S} - -∗
     γ_σ1 ⤳@{m_state m1} - -∗
+    γ_σ2 ⤳@{m_state m2} - -∗
     γ_oe ⤳@{option EV}- -∗
-    (γ_s ⤳ s -∗ γ_σ1 ⤳ σ1 -∗ γ_oe ⤳ Some e -∗ σ2 ≈{m2}≈>ₜ tgt_link_right_constP R Π γ_s γ_σ1 γ_oe) -∗
+    (γ_s ⤳ s -∗ γ_σ1 ⤳ σ1 -∗ γ_oe ⤳ Some e -∗ σ2 ≈{m2}≈>ₜ tgt_link_right_constP R Π γ_s γ_σ1 γ_σ2 γ_oe) -∗
     (MLFRecv SPRight e, s, σ1, σ2) ≈{link_trans R m1 m2}≈>ₜ Π.
   Proof.
-    iIntros "Hγ_s Hγ_σ1 Hγ_oe Hsim".
+    iIntros "Hγ_s Hγ_σ1 Hγ_σ2 Hγ_oe Hsim".
     iMod (mstate_var_split γ_s with "Hγ_s") as "[??]".
     iMod (mstate_var_split γ_σ1 with "Hγ_σ1") as "[??]".
     iMod (mstate_var_split γ_oe with "Hγ_oe") as "[??]".
     iApply sim_tgt_link_recv_right. iSpecialize ("Hsim" with "[$] [$] [$]").
     iApply (sim_gen_wand with "Hsim"). iIntros (??) "Hsim".
-    iApply ("Hsim" with "[$] [$] [$]").
+    iApply ("Hsim" with "[$] [$] [$] [$]").
   Qed.
 
-  Lemma sim_tgt_link_right_const_run γ_s γ_σ1 γ_oe R m1 m2 s σ1 σ2 Π :
+  Lemma sim_tgt_link_right_const_run γ_s γ_σ1 γ_σ2 γ_oe R m1 m2 s σ1 σ2 Π :
     γ_s ⤳@{S} - -∗
     γ_σ1 ⤳@{m_state m1} - -∗
+    γ_σ2 ⤳@{m_state m2} - -∗
     γ_oe ⤳@{option EV}- -∗
-    (γ_s ⤳ s -∗ γ_σ1 ⤳ σ1 -∗ γ_oe ⤳ (@None EV) -∗ σ2 ≈{m2}≈>ₜ tgt_link_right_constP R Π γ_s γ_σ1 γ_oe) -∗
+    (γ_s ⤳ s -∗ γ_σ1 ⤳ σ1 -∗ γ_oe ⤳ (@None EV) -∗ σ2 ≈{m2}≈>ₜ tgt_link_right_constP R Π γ_s γ_σ1 γ_σ2 γ_oe) -∗
     (MLFRun (Some SPRight), s, σ1, σ2) ≈{link_trans R m1 m2}≈>ₜ Π.
   Proof.
-    iIntros "Hγ_s Hγ_σ1 Hγ_oe Hsim".
+    iIntros "Hγ_s Hγ_σ1 Hγ_σ2 Hγ_oe Hsim".
     iMod (mstate_var_split γ_s with "Hγ_s") as "[??]".
     iMod (mstate_var_split γ_σ1 with "Hγ_σ1") as "[??]".
     iMod (mstate_var_split γ_oe with "Hγ_oe") as "[??]".
     iApply sim_tgt_link_run_right. iSpecialize ("Hsim" with "[$] [$] [$]").
     iApply (sim_gen_wand with "Hsim"). iIntros (??) "Hsim".
-    iApply ("Hsim" with "[$] [$] [$]").
+    iApply ("Hsim" with "[$] [$] [$] [$]").
   Qed.
 
 End link.
