dimsum_examples/iris/echo_noloop.v
@@ -385,13 +385,16 @@ Section echo_getc.
     (* Target's spec module (Right linking case - getc) *)
     iMod (mstate_var_alloc (m_state (spec_trans rec_event Z))) as (γt_r) "Hγt_r".
 
+    (* Target's rec module (Left linking case - echo) *)
+    iMod (mstate_var_alloc (m_state rec_trans)) as (γt_l) "Hγt_l".
+
     (* TODO: "queue" for linking?  *)
     iMod (mstate_var_alloc (list seq_product_case)) as (γt_q) "Hγt_q".
 
     (* (* Linking event to pass around *) *)
     iMod (mstate_var_alloc (option rec_ev)) as (γt_oe) "Hγt_oe".
 
-    iApply (sim_tgt_link_left_const_run γt_q γt_r γt_oe with "[$] [$] [$] [-]").
+    iApply (sim_tgt_link_left_const_run γt_q γt_l γt_r γt_oe with "[$] [$] [$] [$] [-]").
     iIntros "Hγt_q Hγt_r Hγt_oe".
 
 
@@ -416,7 +419,7 @@ Section echo_getc.
       (* iDestruct 1 as (?? ->) "[[% [Hγt_oe [Hγt_q Hγt_r]]] HC]" => /=. *)
       iDestruct 1 as (?? ->) "[[% [Hγt_oe [Hγt_q Hγt_r]]] HC]" => /=.
 
-      iIntros "%%% Hγt_q' Hγt_r' Hγt_oe'".
+      iIntros "%%% Hγt_q' Hγt_l Hγt_r' Hγt_oe'".
 
       iDestruct (mstate_var_merge with "Hγt_r Hγt_r'") as "[<- Hγt_r]".
       iDestruct (mstate_var_merge with "Hγt_oe Hγt_oe'") as "[<- Hγt_oe]".
@@ -427,22 +430,23 @@ Section echo_getc.
       iApply (sim_tgt_link_run_right with "[-]"). iApply "HC". iSplit!.
       iIntros (??). iDestruct 1 as (??) "[% HC]" => /=. simplify_eq.
       iIntros (??????). destruct!/=.
-      iApply (sim_tgt_link_left_const_recv γt_q γt_r γt_oe with "[$] [Hγt_r] [$] [-]"). 1: done.
+      iApply (sim_tgt_link_left_const_recv γt_q γt_l γt_r γt_oe with "[$] [Hγt_l] [Hγt_r] [$] [-]"). 1-2: done.
       iIntros "Hγt_q Hγt_r Hγt_oe".
       iApply "HC". iSplit!.
       iIntros (??). iDestruct 1 as (? ->) "HC" => /=.
-      iIntros "%%% Hγt_q' Hγt_r' Hγt_oe'".
+      iIntros "%%% Hγt_q' Hγt_l Hγt_r' Hγt_oe'".
       iDestruct (mstate_var_merge with "Hγt_r Hγt_r'") as "[<- Hγt_r]".
       iDestruct (mstate_var_merge with "Hγt_oe Hγt_oe'") as "[<- Hγt_oe]".
       iDestruct (mstate_var_merge with "Hγt_q Hγt_q'") as "[<- Hγt_q]". iIntros (?). simplify_eq.
-      iApply (sim_tgt_link_left_const_run γt_q γt_r γt_oe with "[$] [Hγt_r] [$] [-]"). 1: done.
+
+      iApply (sim_tgt_link_left_const_run γt_q γt_l γt_r γt_oe with "[$] [Hγt_l] [Hγt_r] [$] [-]"). 1-2: done.
       iIntros "Hγt_q Hγt_r Hγt_oe".
       iApply ("HC" with "[-]"). iSplit!. iFrame.
     }
     iSplit!.
     iSplitL.
     - iIntros (??) "[% [% [% [% [% [Hγs [Hγt_oe [Hγt_q [Hγt_r [% HC]]]]]]]]]]" => /=.
-      subst. iIntros (???) "Hγt_q' Hγt_r' Hγt_oe'".
+      subst. iIntros (???) "Hγt_q' Hγt_l Hγt_r' Hγt_oe'".
 
       iDestruct (mstate_var_merge with "Hγt_r Hγt_r'") as "[<- Hγt_r]".
       iDestruct (mstate_var_merge with "Hγt_oe Hγt_oe'") as "[<- Hγt_oe]".
@@ -465,18 +469,18 @@ Section echo_getc.
       iApply "HC". iSplit!. iIntros (??). iDestruct 1 as (?? -> ->) "HC".
       iApply (sim_src_constP_next with "[Hγt] [Hγκ] [Hγs] [%] [-]"); [done..|].
       iIntros "Hγs". destruct!/=.
-      iApply (sim_tgt_link_left_const_recv γt_q γt_r γt_oe with "[$] [Hγt_r] [$] [-]"). 1: done.
+      iApply (sim_tgt_link_left_const_recv γt_q γt_l γt_r γt_oe with "[$] [Hγt_l][Hγt_r] [$] [-]"). 1-2: done.
       iIntros "Hγt_q Hγt_r Hγt_oe".
       iApply ("HC" with "[-]"). iFrame. iSplit!.
       iIntros (??). iDestruct 1 as (? ->) "HC".
-      iIntros (???) "Hγt_q' Hγt_r' Hγt_oe'".
+      iIntros (???) "Hγt_q' Hγt_l Hγt_r' Hγt_oe'".
 
       iDestruct (mstate_var_merge with "Hγt_r Hγt_r'") as "[<- Hγt_r]".
       iDestruct (mstate_var_merge with "Hγt_oe Hγt_oe'") as "[<- Hγt_oe]".
       iDestruct (mstate_var_merge with "Hγt_q Hγt_q'") as "[<- Hγt_q]".
       iIntros (?). simplify_eq.
 
-      iApply (sim_tgt_link_left_const_run γt_q γt_r γt_oe with "[$] [Hγt_r] [$] [-]"). 1: done.
+      iApply (sim_tgt_link_left_const_run γt_q γt_l γt_r γt_oe with "[$] [Hγt_l] [Hγt_r] [$] [-]"). 1-2: done.
       iIntros "???".
 
       iApply "HC". iSplit!. iFrame.
